Update Submission.thy

homework/09/Submission.thy
@@ -13,21 +13,107 @@ If: "\<lbrakk> \<turnstile>{I} {\<lambda>s. P s \<and> bval b s} c\<^sub>1 {Q}; 
      \<Longrightarrow> \<turnstile>{I} {P} IF b THEN c\<^sub>1 ELSE c\<^sub>2 {Q}"  |
 conseq: "\<lbrakk> \<forall>s. P' s \<longrightarrow> P s;  \<turnstile>{I} {P} c {Q};  \<forall>s. Q s \<longrightarrow> Q' s \<rbrakk>
         \<Longrightarrow> \<turnstile>{I} {P'} c {Q'}" |
-While: "\<turnstile>{I} {\<lambda>s. P s \<and> bval b s} c {P} \<Longrightarrow>
+While: "\<turnstile>{P} {\<lambda>s. P s \<and> bval b s} c {\<lambda>s. P s} \<Longrightarrow>
         \<turnstile>{I} {P} WHILE b DO c {\<lambda>s. P s \<and> \<not> bval b s}"  |
-Continue: ""
+Continue: "\<turnstile>{I} {I} CONTINUE {P}"
 \<comment> \<open>Add your cases here\<close>
-theorem hoare_sound: "\<turnstile>{I} {P}c{Q} \<Longrightarrow> \<Turnstile>\<^sub>c{I} {P}c{Q}"
-  sorry
+
+lemmas [simp] = hoare.Skip hoare.Assign hoare.Seq If
+
+lemmas [intro!] = hoare.Skip hoare.Assign hoare.Seq hoare.If
+
+lemma strengthen_pre:
+  "\<lbrakk> \<forall>s. P' s \<longrightarrow> P s;  \<turnstile>{I} {P} c {Q} \<rbrakk> \<Longrightarrow> \<turnstile>{I} {P'} c {Q}"
+by (blast intro: conseq)
+
+lemma weaken_post:
+  "\<lbrakk> \<turnstile>{I} {P} c {Q};  \<forall>s. Q s \<longrightarrow> Q' s \<rbrakk> \<Longrightarrow>  \<turnstile>{I} {P} c {Q'}"
+  by (blast intro: conseq)
+
+theorem hoare_sound: "\<turnstile>{I} {P} c {Q} \<Longrightarrow> \<Turnstile>\<^sub>c{I} {P} c {Q}"
+proof(induction rule: hoare.induct)
+  case (While P b c I)
+  have "(WHILE b DO c,s) \<Rightarrow> (f, t)  \<Longrightarrow>  P s  \<Longrightarrow>  P t \<and> \<not> bval b t" for s f t
+  proof(induction "WHILE b DO c" s f t rule: big_step_induct)
+    case WhileFalse thus ?case by blast
+  next
+    case WhileTrue thus ?case
+      using While.IH unfolding hoare_valid_def
+      by (simp add: hoare_valid\<^sub>c_def)
+  qed
+  moreover have "(WHILE b DO c,s) \<Rightarrow> (f, t) \<Longrightarrow> f = False" for s f t
+   proof(induction "WHILE b DO c" s f t rule: big_step_induct)
+    case WhileFalse thus ?case by blast
+  next
+    case WhileTrue thus ?case
+      using While.IH unfolding hoare_valid_def
+      by (simp add: hoare_valid\<^sub>c_def)
+  qed
+  ultimately show ?case unfolding hoare_valid\<^sub>c_def by fastforce
+qed (fastforce simp: hoare_valid\<^sub>c_def)+
+
+lemma Assign': "\<forall>s. P s \<longrightarrow> Q(s[a/x]) \<Longrightarrow> \<turnstile>{I} {P} x ::= a {Q}"
+by (simp add: strengthen_pre[OF _ Assign])
+
+lemma While':
+assumes "\<turnstile>{P} {\<lambda>s. P s \<and> bval b s} c {P}" and "\<forall>s. P s \<and> \<not> bval b s \<longrightarrow> Q s"
+shows "\<turnstile>{I} {P} WHILE b DO c {Q}"
+by(rule weaken_post[OF While[OF assms(1)] assms(2)])
 
 definition wp :: "com \<Rightarrow> assn \<Rightarrow> assn \<Rightarrow> assn"  where
-  "wp _ = undefined"
+  "wp c I Q = (\<lambda>s. \<forall>f t. (c,s) \<Rightarrow> (f, t)  \<longrightarrow>  (if f then I t else Q t))"
+
+lemma wp_SKIP[simp]: "wp SKIP I Q = Q"
+by (rule ext) (auto simp: wp_def)
+
+lemma wp_Ass[simp]: "wp (x::=a) I Q = (\<lambda>s. Q(s[a/x]))"
+by (rule ext) (auto simp: wp_def)
+
+lemma wp_Seq[simp]: "wp (c\<^sub>1;;c\<^sub>2) I Q = wp c\<^sub>1 I (wp c\<^sub>2 I Q)"
+by (rule ext) (auto simp: wp_def)
+
+lemma wp_If[simp]:
+ "wp (IF b THEN c\<^sub>1 ELSE c\<^sub>2) I Q =
+ (\<lambda>s. if bval b s then wp c\<^sub>1 I Q s else wp c\<^sub>2 I Q s)"
+by (rule ext) (auto simp: wp_def)
+
+lemma wp_While_True[simp]: "bval b s \<Longrightarrow>
+  wp (WHILE b DO c) I Q s = wp c (wp (WHILE b DO c) I Q) (wp (WHILE b DO c) I Q) s"
+using WhileTrue wp_def by auto
+
+lemma wp_While_False[simp]: "\<not> bval b s \<Longrightarrow> wp (WHILE b DO c) I Q s = Q s"
+  using WhileFalse wp_def by auto
+
+lemma wp_Continue[simp]: "wp (CONTINUE) I Q = I"
+  using wp_def by auto
+
+lemma wp_is_pre: "\<turnstile>{I} {wp c I Q} c {Q}"
+proof(induction c arbitrary: I Q)
+  case If thus ?case
+    by (smt (z3) conseq hoare.If wp_If)
+next
+  case (While b c)
+  let ?w = "WHILE b DO c"
+  show "\<turnstile>{I} {wp ?w I Q} ?w {Q}"
+  proof(rule While')
+    show "\<turnstile>{wp ?w I Q} {\<lambda>s. wp ?w I Q s \<and> bval b s} c {wp ?w I Q}"
+    proof(rule strengthen_pre[OF _ While.IH])
+      show "\<forall>s. wp ?w I Q s \<and> bval b s \<longrightarrow> wp c (wp ?w I Q) (wp ?w I Q) s" by auto
+    qed
+    show "\<forall>s. wp ?w I Q s \<and> \<not> bval b s \<longrightarrow> Q s" by auto
+  qed
+next case CONTINUE show ?case by (simp add: hoare.Continue)
+qed auto
 
 lemma hoare_complete: assumes "\<Turnstile> {P}c{Q}"
   shows "\<turnstile>{Q} {P}c{Q}"
-  sorry
+proof(rule strengthen_pre)
+  show "\<forall>s. P s \<longrightarrow> wp c Q Q s" using assms
+    by (auto simp: hoare_valid_def wp_def)
+  show "\<turnstile>{Q} {wp c Q Q} c {Q}" by(rule wp_is_pre)
+qed
 
 theorem hoare_sound_complete: "\<turnstile>{Q} {P}c{Q} \<longleftrightarrow> \<Turnstile> {P}c{Q}"
-  sorry
+  by (metis hoare_complete hoare_sound hoare_valid\<^sub>c_def hoare_valid_def)
 
 end
